\documentclass[a4paper,12pt]{article}
\begin{document}
Note $\psi = (1 - \sqrt{5})/2$.
Let's show by induction that,
\[ Fib(n) = (\phi^n - \psi^n)/\sqrt{5}.\]
If $n = 0$, we have
\[ Fib(0) = 0 = (\phi^0 - \psi^0)/\sqrt{5}.\]
and if $n = 1$,
\[ Fib(1) = 1 = (\phi - \psi)/\sqrt{5}.\]
Suppose the property is verified the interges $n$ and $n+1$ where $n
\ge 0$.  By induction we have,
\begin{eqnarray*}
Fib(n+2) &=& Fib(n+1) + Fib(n) \\ &=&
(\phi^{n+1} - \psi^{n+1})/\sqrt{5} +
(\phi^n - \psi^n)/\sqrt{5} \\ &=&
(\phi^n(1 + \phi) - \psi^n(1 + \psi))/\sqrt{5}
\end{eqnarray*}
Given that $\psi$ and $\phi$ and the solutions of the equations $x^2 =
x + 1$, we have the desired result.

\medskip
So we have the equality
\[ Fib(n) = (\phi^n - \psi^n)/\sqrt{5}.\]
Given that we have
\[ 2 < \sqrt{5} < 3.\]
We then deduce that
\[ -1 < \psi < 0.\]
Thus,
\[ \left|\frac{\psi^n}{\sqrt{5}}\right| < \frac{1}{\sqrt5} <
\frac{1}{2}.\]
And finally,
\[ Fib(n) - \frac{1}{2} < \frac{\phi^n}{\sqrt{5}} <
Fib(n) + \frac{1}{2}.\]
So we have the desired result.
\end{document}
